finished main results

theories/FOL/Util/Friedman.v
@@ -2,15 +2,27 @@ Require Import List Lia.
 From Undecidability.FOL.Util Require Import Syntax Syntax_facts FullTarski FullTarski_facts FullDeduction_facts FullDeduction.
 Import Vector.VectorNotations.
 
+
+
+
+Lemma size_rect {X} σ f : 
+  (forall x, (forall y : X, σ y < σ x -> f y) -> f x) -> forall x, f x.
+Proof.
+  intros H x. apply H.
+  induction (σ x).
+  - intros y. now intros F % PeanoNat.Nat.nlt_0_r. 
+  - intros y Hy. apply H.
+    intros z Hz. apply IHn. lia.
+Defined.
+
+
+
 Section Signature.
 
   
  (* Assume some signature and corresponding arity functions *)
  Context {Σ_funcs : funcs_signature}.
  Context {Σ_preds : preds_signature}.
- 
- Variable Σ_funcs_ar : Σ_funcs -> nat.
- Variable Σ_preds_ar : Σ_preds -> nat.
 
  
 Section Expanded.
@@ -23,28 +35,29 @@ Section Expanded.
   Definition new_preds_ar (P : new_preds) :=
     match P with
     | Q_ => 0
-    | old_preds P => Σ_preds_ar P
+    | old_preds P => ar_preds P
     end.
 
   Instance funcs_signature : funcs_signature :=
-    {| syms := Σ_funcs ; ar_syms := Σ_funcs_ar |}.
+    {| syms := Σ_funcs ; ar_syms := ar_syms |}.
 
   Instance preds_signature : preds_signature :=
     {| preds := new_preds ; ar_preds := new_preds_ar |}.
 
 
   Definition Q {ff} := (@atom funcs_signature preds_signature _ ff Q_ ([])).
-  Definition dnQ {ff} phi : form := (phi ~> @Q ff) ~> Q.
+  Definition dn {ff} F phi : @form funcs_signature preds_signature _ ff :=
+    (phi ~> F) ~> F.
 
   Fixpoint Friedman {ff} (phi : @form funcs_signature preds_signature _ ff) : form ff :=
     match phi with
     | falsity => Q
-    | atom P v => match P with Q_ => Q | _ => dnQ (atom P v) end
+    | atom P v => match P with Q_ => Q | _ => dn Q (atom P v) end
     | bin Impl phi psi => (Friedman phi) ~> (Friedman psi)
     | bin Conj phi psi => (Friedman phi) ∧ (Friedman psi)
-    | bin Disj phi psi => dnQ ((Friedman phi) ∨ (Friedman psi))
+    | bin Disj phi psi => dn Q ((Friedman phi) ∨ (Friedman psi))
     | quant All phi => ∀ (Friedman phi)
-    | quant Ex phi => dnQ (∃ (Friedman phi))
+    | quant Ex phi => dn Q (∃ (Friedman phi))
     end.
 
                       
@@ -52,21 +65,157 @@ Section Expanded.
   
   Definition List_Fr {ff} Gamma := map (@Friedman ff) Gamma.
   
-  Lemma subst_Fr {ff} (phi : @form funcs_signature preds_signature _ ff) sigma:
+  Fact subst_Fr {ff} (phi : @form funcs_signature preds_signature _ ff) sigma:
     subst_form sigma (Fr phi) = Fr (subst_form sigma phi).
   Proof.
     revert sigma.
     induction phi; cbn.
     - reflexivity.
     - destruct P; reflexivity.
-    - destruct b0; cbn; unfold dnQ, Q; congruence.
-    - destruct q; cbn; intros sigma; unfold dnQ, Q; congruence.
+    - destruct b0; cbn; unfold dn, Q; congruence.
+    - destruct q; cbn; intros sigma; unfold dn, Q; congruence.
   Qed.
-  
-  
-  Lemma DNE_Q {ff} Gamma phi : Gamma ⊢I Fr (dnQ phi) ~> @Friedman ff phi. 
-  Proof. Admitted.
 
+  Fact subst_List_Fr {ff} L sigma :
+    map (subst_form sigma) (map (@Friedman ff) L) = map Friedman (map (subst_form sigma) L).
+  Proof.
+    induction L.
+    - reflexivity.
+    - cbn. now rewrite IHL, subst_Fr.
+  Qed.
+
+  Lemma Fr_dn {ff} Gamma phi :
+    Gamma ⊢I Fr (@dn ff Q phi) <-> Gamma ⊢I dn Q (Fr phi).
+  Proof.
+  Admitted.
+      
+
+  Lemma double_dn {ff} Gamma F phi :
+    Gamma ⊢I @dn ff F (dn F phi) ~> dn F phi.
+  Proof.
+    apply II, II. eapply IE with (phi0:= _ ~> _).
+    { apply Ctx; firstorder. }
+    apply II. apply IE with (phi0:= phi ~> F).
+    all: apply Ctx; firstorder.
+  Qed.
+
+  Lemma rm_dn {ff} Gamma F alpha beta :
+    (alpha :: Gamma) ⊢I beta -> (@dn ff F alpha :: Gamma) ⊢I dn F beta.
+  Proof.
+    intros H.
+    apply II. eapply IE with (phi:= _ ~> _).
+    { apply Ctx; firstorder. }
+    apply II. eapply IE with (phi:= beta).
+    {apply Ctx; firstorder. }
+    eapply Weak; [eassumption|firstorder].
+  Qed.
+
+
+  
+  Lemma form_up_var0_invar {ff} (phi : @form _ _ _ ff) :
+    phi[up ↑][$0..] = phi.
+  Proof.
+  Admitted.                             
+  
+  Lemma dn_forall {ff} Gamma phi :
+    Gamma ⊢I @dn ff Q (∀ phi) ~> ∀ dn Q phi.
+  Proof.
+    apply II. constructor. apply II.
+    cbn; fold Q.
+    change ((∀ phi[up ↑])) with ((∀ phi)[↑]).
+    eapply IE with (phi0:= _ ~> _).
+    { apply Ctx; firstorder. }
+    apply II.
+    eapply IE with (phi0:= phi).
+    { apply Ctx; firstorder. }
+    cbn. rewrite <-form_up_var0_invar.
+    apply AllE, Ctx; firstorder.
+  Qed.
+      
+  
+  Fixpoint form_size {ff} (phi : @form funcs_signature preds_signature _ ff) :=
+    match phi with
+    | falsity => 0
+    | atom P v => 1
+    | bin _ phi psi => S (form_size phi + form_size psi)
+    | quant _ phi => S (form_size phi)
+    end.
+
+  Lemma DNE_Fr {ff} :
+    forall phi Gamma, Gamma ⊢I Fr (dn Q phi) ~> @Friedman ff phi. 
+  Proof.
+    refine (size_rect form_size _ _). intros phi sRec.
+    destruct phi; intros Gamma.
+    - apply II. eapply IE; cbn.
+      { apply Ctx; firstorder. }
+      apply II, Ctx; firstorder.
+    - destruct P.
+      + apply II. eapply IE; cbn.
+        {apply Ctx; firstorder. }
+        apply II, Ctx; firstorder.
+      + apply double_dn.
+    - destruct b0; cbn.
+      + apply II, CI.
+        * eapply IE. apply sRec.
+          {cbn; lia. }
+          cbn; apply rm_dn.
+          eapply CE1, Ctx; firstorder.
+        * eapply IE. apply sRec.
+          {cbn; lia. }
+          cbn; apply rm_dn.
+          eapply CE2, Ctx; firstorder.
+      + apply double_dn.
+      + apply II, II. eapply IE.
+        apply sRec.
+        {cbn; lia. }
+        cbn; apply II. eapply IE with (phi:= _ ~> _).
+        { apply Ctx; firstorder. }
+        apply II. eapply IE with (phi:= Fr phi2).
+        { apply Ctx; firstorder. }
+        eapply IE with (phi:= Fr phi1); apply Ctx; firstorder.
+    - destruct q.
+      + cbn. apply II. apply IE with (phi0:= ∀ Fr (dn Q phi)).
+        { apply II. constructor. cbn; fold Q.
+          eapply IE. apply sRec; auto.
+          rewrite <-form_up_var0_invar.
+          apply AllE, Ctx. firstorder. }
+        constructor. apply Fr_dn.
+        cbn; fold Q. rewrite <- form_up_var0_invar.
+        apply AllE. cbn; fold Q.
+        apply imps, dn_forall.
+      + apply double_dn.
+  Qed.
+    
+  Lemma Expl_Fr {ff} Gamma phi : Gamma ⊢I Q ~> @Friedman ff phi.
+  Proof.
+    induction phi; cbn; apply II.
+    - apply Ctx; firstorder.
+    - destruct  P.
+      + apply Ctx; firstorder.
+      + apply II, Ctx; firstorder.
+    - destruct b0.
+      + apply CI; now apply imps.
+      + apply II, Ctx; firstorder.
+      + apply II. eapply IE. apply IHphi2.
+        apply Ctx; firstorder.
+    - destruct q.
+      + constructor. apply imps, IHphi.
+      + apply II, Ctx; firstorder.
+  Qed.          
+  
+  Lemma Peirce_Fr {ff} Gamma phi psi : Gamma ⊢I @Friedman ff (((phi ~> psi) ~> phi) ~> phi).
+  Proof.
+    eapply IE. apply DNE_Fr. cbn.
+    apply II. eapply IE.
+    { apply Ctx; firstorder. }
+    apply II. eapply IE.
+    { apply Ctx; firstorder. }
+    apply II. eapply IE; [apply Expl_Fr|].
+    eapply IE.
+    { apply Ctx; firstorder. }
+    apply II. apply Ctx; firstorder.
+  Qed.
+    
   
   Lemma Friedman_cl_to_intu {ff} Gamma phi :
     Gamma ⊢C phi -> (List_Fr Gamma) ⊢I @Friedman ff phi.
@@ -74,7 +223,7 @@ Section Expanded.
     intros H. induction H; unfold List_Fr in *.
     - cbn. now constructor.
     - econstructor; eassumption.
-    - cbn. constructor. admit.
+    - cbn. constructor. now rewrite subst_List_Fr.
     - cbn in *. eapply AllE with (t0:=t) in IHprv.
       cbn in *. now rewrite subst_Fr in IHprv. 
     - cbn. apply II.
@@ -82,9 +231,20 @@ Section Expanded.
       + apply Ctx. firstorder.
       + apply Weak with (A0 := map Friedman A); [|firstorder].
         apply ExI with (t0:=t). now rewrite subst_Fr.
-    - admit.
     - cbn in *.
-      specialize (DNE_Q (map Friedman A) phi) as H'.
+      eapply IE. apply DNE_Fr. unfold dn in *; cbn.
+      apply II. eapply IE.
+      { eapply Weak; [apply IHprv1|firstorder]. }
+      apply II. eapply IE.
+      { apply Ctx; firstorder. }
+      rewrite <-subst_Fr, <-subst_List_Fr in IHprv2.
+      eapply ExE.
+      { apply Ctx; firstorder. }
+      cbn. eapply Weak.
+      + apply IHprv2.
+      + firstorder.
+    - cbn in *.
+      specialize (DNE_Fr phi (map Friedman A)) as H'.
       eapply IE; [eassumption|].
       cbn; apply II. eapply Weak; eauto.
     - now apply Ctx, in_map.
@@ -97,10 +257,19 @@ Section Expanded.
     - cbn. apply II. eapply IE.
       + apply Ctx. firstorder.
       + apply DI2. eapply Weak; eauto.
-    - cbn in *. admit.
-    - specialize (DNE_Q (map Friedman A) (((phi ~> psi) ~> phi) ~> phi)) as H'.
-      eapply IE; [eassumption|]. cbn. apply gen_peirce.
-  Admitted.
+    - eapply IE. apply DNE_Fr.
+      cbn in *.
+      apply II. eapply IE.
+      { eapply Weak; [apply IHprv1|firstorder]. }
+      apply II. eapply IE.
+      { apply Ctx; firstorder. }
+      apply imps in IHprv2.
+      apply imps in IHprv3.
+      eapply DE.
+      1 : apply Ctx; firstorder.
+      1,2 : apply imps; eapply Weak; [eassumption|firstorder].
+    - apply Peirce_Fr.
+  Qed.
 
     
 End Expanded.
